Getting EVAL to deal with wordn properly. Have exchanged applications of Define for new_definition, so the definitions are not automatically added to the global compset. Then the rewrites used by WORD_CONV are added to the global compset. Note: you need to load wordnLib in order to get the global compset updated for wordn.

src/n_bit/bitsLib.sml
@@ -40,18 +40,21 @@ fun cbv_LOG2_CONV tm =
       | Domain => raise (mk_HOL_ERR "bitsLib" "cbv_LOG2" "")
 *)
 
+val thms = 
+  [numeralTheory.numeral_funpow, pairTheory.UNCURRY_DEF,
+   iBITWISE, NUMERAL_BITWISE, NUMERAL_DIV2, SIGN_EXTEND_def,
+   DIVMOD_2EXP, iMOD_2EXP, NUMERAL_MOD_2EXP, NUMERAL_DIV_2EXP, TIMES_2EXP_def,
+   LSBn_def, BITV_def, SBIT_def,
+   NUMERAL_ONLY_RULE [NUMERAL_DIV_2EXP,iMOD_2EXP] `n` BITS_def,
+   NUMERAL_ONLY_RULE [NUMERAL_DIV_2EXP,iMOD_2EXP] `n` SLICE_def,
+   NUMERAL_ONLY_RULE [BITS_ZERO2] `n`  BIT_def,
+   numeral_log2,numeral_ilog2
+  ] ;
+
 fun bits_compset () =
   let val compset = reduceLib.num_compset()
-      val _ = add_thms
-                [numeralTheory.numeral_funpow, pairTheory.UNCURRY_DEF,
-                 iBITWISE, NUMERAL_BITWISE, NUMERAL_DIV2, SIGN_EXTEND_def,
-                 DIVMOD_2EXP, iMOD_2EXP, NUMERAL_MOD_2EXP, NUMERAL_DIV_2EXP, TIMES_2EXP_def,
-                 LSBn_def, BITV_def, SBIT_def,
-                 NUMERAL_ONLY_RULE [NUMERAL_DIV_2EXP,iMOD_2EXP] `n` BITS_def,
-                 NUMERAL_ONLY_RULE [NUMERAL_DIV_2EXP,iMOD_2EXP] `n` SLICE_def,
-                 NUMERAL_ONLY_RULE [BITS_ZERO2] `n`  BIT_def,
-                 numeral_log2,numeral_ilog2
-                 ] compset
+      val _ = add_thms thms compset
+      val _ = add_thms thms computeLib.the_compset
    (*   val _ = add_conv (``$LOG2``, 1, cbv_LOG2_CONV) compset *)
 in
   compset
